fstar/common/proofs/MLS.Crypto.Derived.Lemmas.fst
@@ -1,0 +1,13 @@
+module MLS.Crypto.Derived.Lemmas
+
+open MLS.Crypto.Derived
+
+#push-options "--fuel 0 --ifuel 0"
+
+val get_mls_label_inj:
+  l1:valid_label -> l2:valid_label ->
+  Lemma
+  (requires get_mls_label l1 == get_mls_label l2)
+  (ensures l1 == l2)
+let get_mls_label_inj l1 l2 =
+  String.concat_injective "MLS 1.0 " "MLS 1.0 " l1 l2
