fstar/common/symbolic/MLS.Crypto.Derived.Symbolic.SignWithLabel.fst
@@ -1,0 +1,211 @@
+module MLS.Crypto.Derived.Symbolic.SignWithLabel
+
+open Comparse
+open DY.Core
+open DY.Lib
+open MLS.NetworkTypes
+open MLS.Crypto
+open MLS.Crypto.Derived.Lemmas
+open MLS.Symbolic
+open MLS.Result
+
+#push-options "--fuel 0 --ifuel 0"
+
+(*** Split predicate for SignWithLabel ***)
+
+noeq
+type signwithlabel_crypto_pred {|crypto_usages|} = {
+  pred: trace -> vk:bytes{SigKey? (get_signkey_usage vk)} -> msg:bytes -> prop;
+  pred_later:
+    tr1:trace -> tr2:trace ->
+    vk:bytes{SigKey? (get_signkey_usage vk)} -> msg:bytes ->
+    Lemma
+    (requires pred tr1 vk msg /\ tr1 <$ tr2)
+    (ensures pred tr2 vk msg)
+  ;
+}
+
+let split_signwithlabel_crypto_pred_params {|crypto_usages|}: split_function_parameters = {
+  tag_set_t = valid_label;
+  tag_t = mls_ascii_string;
+  is_disjoint = unequal;
+  tag_belong_to = (fun tag tag_set ->
+    tag = get_mls_label tag_set
+  );
+  cant_belong_to_disjoint_sets = (fun tag tag_set_1 tag_set_2 ->
+    FStar.Classical.move_requires_2 get_mls_label_inj tag_set_1 tag_set_2
+  );
+
+  tagged_data_t = (trace & (vk:bytes{SigKey? (get_signkey_usage vk)}) & bytes);
+  raw_data_t = (trace & (vk:bytes{SigKey? (get_signkey_usage vk)}) & bytes);
+  output_t = prop;
+
+  decode_tagged_data = (fun (tr, vk, data) -> (
+    match parse (sign_content_nt bytes) data with
+    | Some ({label; content}) -> Some (label, (tr, vk, content))
+    | None -> None
+  ));
+
+  local_fun_t = signwithlabel_crypto_pred;
+  global_fun_t = trace -> vk:bytes{SigKey? (get_signkey_usage vk)} -> bytes -> prop;
+
+  default_global_fun = (fun tr vk content -> False);
+
+
+  apply_local_fun = (fun pred (tr, vk, content) -> pred.pred tr vk content);
+  apply_global_fun = (fun pred (tr, vk, msg) -> pred tr vk msg);
+  mk_global_fun = (fun pred tr vk msg -> pred (tr, vk, msg));
+  apply_mk_global_fun = (fun _ _ -> ());
+}
+
+#push-options "--ifuel 1"
+val has_signwithlabel_pred: {|cusgs:crypto_usages|} -> sign_crypto_predicate cusgs -> (valid_label & signwithlabel_crypto_pred) -> prop
+let has_signwithlabel_pred #cusgs sign_pred (lab, local_pred) =
+  forall tr vk msg.
+    {:pattern sign_pred.pred tr vk msg}
+    match parse (sign_content_nt bytes) msg with
+    | Some {label; content} -> (
+      label == get_mls_label lab ==> (
+        sign_pred.pred tr vk msg ==
+        local_pred.pred tr vk content
+      )
+    )
+    | _ -> True
+#pop-options
+
+val intro_has_signwithlabel_pred:
+  {|cusgs:crypto_usages|} ->
+  sign_pred:sign_crypto_predicate cusgs -> tagged_local_pred:(valid_label & signwithlabel_crypto_pred) ->
+  Lemma
+  (requires has_local_fun split_signwithlabel_crypto_pred_params sign_pred.pred tagged_local_pred)
+  (ensures has_signwithlabel_pred sign_pred tagged_local_pred)
+let intro_has_signwithlabel_pred #cusgs sign_pred (tag, local_pred) =
+  introduce
+    forall tr vk msg.
+      match parse (sign_content_nt bytes) msg with
+      | Some {label; content} -> (
+        label == get_mls_label tag ==> (
+          sign_pred.pred tr vk msg ==
+          local_pred.pred tr vk content
+        )
+      )
+      | _ -> True
+  with (
+    has_local_fun_elim split_signwithlabel_crypto_pred_params sign_pred.pred tag local_pred (tr, vk, msg)
+  )
+
+val mk_global_mls_sign_pred:
+  {|crypto_usages|} ->
+  list (valid_label & signwithlabel_crypto_pred) ->
+  trace -> vk:bytes{SigKey? (get_signkey_usage vk)} -> bytes ->
+  prop
+let mk_global_mls_sign_pred tagged_local_preds vk msg =
+  mk_global_fun split_signwithlabel_crypto_pred_params tagged_local_preds vk msg
+
+#push-options "--ifuel 2"
+val mk_global_mls_sign_pred_later:
+  {|crypto_usages|} ->
+  tagged_local_preds:list (valid_label & signwithlabel_crypto_pred) ->
+  tr1:trace -> tr2:trace ->
+  vk:bytes{SigKey? (get_signkey_usage vk)} -> msg:bytes ->
+  Lemma
+  (requires
+    mk_global_mls_sign_pred tagged_local_preds tr1 vk msg /\
+    tr1 <$ tr2
+  )
+  (ensures mk_global_mls_sign_pred tagged_local_preds tr2 vk msg)
+let mk_global_mls_sign_pred_later tagged_local_preds tr1 tr2 vk msg =
+  mk_global_fun_eq split_signwithlabel_crypto_pred_params tagged_local_preds (tr1, vk, msg);
+  mk_global_fun_eq split_signwithlabel_crypto_pred_params tagged_local_preds (tr2, vk, msg);
+  introduce forall lpred content. split_signwithlabel_crypto_pred_params.apply_local_fun lpred (tr1, vk, content) ==> split_signwithlabel_crypto_pred_params.apply_local_fun lpred (tr2, vk, content) with (
+    introduce _ ==> _ with _. lpred.pred_later tr1 tr2 vk content
+  )
+#pop-options
+
+val mk_mls_sign_pred:
+  {|cusgs:crypto_usages|} ->
+  list (valid_label & signwithlabel_crypto_pred) ->
+  sign_crypto_predicate cusgs
+let mk_mls_sign_pred #cusgs tagged_local_preds = {
+  pred = mk_global_mls_sign_pred tagged_local_preds;
+  pred_later = mk_global_mls_sign_pred_later tagged_local_preds;
+}
+
+#push-options "--ifuel 1"
+val mk_mls_sign_pred_correct:
+  {|cusgs:crypto_usages|} ->
+  sign_pred:sign_crypto_predicate cusgs -> tagged_local_preds:list (valid_label & signwithlabel_crypto_pred) ->
+  Lemma
+  (requires
+    sign_pred == mk_mls_sign_pred tagged_local_preds /\
+    List.Tot.no_repeats_p (List.Tot.map fst tagged_local_preds)
+  )
+  (ensures for_allP (has_signwithlabel_pred sign_pred) tagged_local_preds)
+let mk_mls_sign_pred_correct sign_pred tagged_local_preds =
+  for_allP_eq (has_signwithlabel_pred sign_pred) tagged_local_preds;
+  no_repeats_p_implies_for_all_pairsP_unequal (List.Tot.map fst tagged_local_preds);
+  FStar.Classical.forall_intro_2 (FStar.Classical.move_requires_2 (mk_global_fun_correct split_signwithlabel_crypto_pred_params tagged_local_preds));
+  FStar.Classical.forall_intro (FStar.Classical.move_requires (intro_has_signwithlabel_pred sign_pred))
+#pop-options
+
+(*** ***)
+
+val has_mls_signwithlabel_pred: {|crypto_invariants|} -> (valid_label & signwithlabel_crypto_pred) -> prop
+let has_mls_signwithlabel_pred #cinvs tagged_local_pred =
+  exists mls_sign_pred.
+    has_sign_predicate cinvs ("MLS.LeafSignKey", mls_sign_pred) /\
+    has_signwithlabel_pred mls_sign_pred tagged_local_pred
+
+(*** Lemmas on SignWithLabel and VerifyWithLabel ***)
+
+val bytes_invariant_sign_with_label:
+  {|crypto_invariants|} -> spred:signwithlabel_crypto_pred -> tr:trace ->
+  sk:bytes -> lab:valid_label -> msg:mls_bytes bytes -> nonce:sign_nonce bytes ->
+  Lemma
+  (requires
+    bytes_invariant tr sk /\
+    bytes_invariant tr nonce /\
+    bytes_invariant tr msg /\
+    get_usage sk == SigKey "MLS.LeafSignKey" empty /\
+    SigNonce? (get_usage nonce) /\
+    (get_label sk) `can_flow tr` (get_label nonce) /\
+    spred.pred tr (vk sk) msg /\
+    has_mls_signwithlabel_pred (lab, spred)
+  )
+  (ensures
+    bytes_invariant tr (Success?.v (sign_with_label sk lab msg nonce)) /\
+    (get_label (Success?.v (sign_with_label sk lab msg nonce))) `can_flow tr` (get_label msg)
+  )
+let bytes_invariant_sign_with_label #ci spred tr sk lab msg nonce =
+  let sign_content: sign_content_nt bytes = {
+    label = get_mls_label lab;
+    content = msg;
+  } in
+  serialize_wf_lemma (sign_content_nt bytes) (bytes_invariant tr) sign_content;
+  serialize_wf_lemma (sign_content_nt bytes) (is_knowable_by (get_label msg) tr) sign_content
+
+val bytes_invariant_verify_with_label:
+  {|ci:crypto_invariants|} -> spred:signwithlabel_crypto_pred -> tr:trace ->
+  vk:bytes -> lab:valid_label -> content:mls_bytes bytes -> signature:bytes ->
+  Lemma
+  (requires
+    bytes_invariant tr vk /\
+    bytes_invariant tr content /\
+    bytes_invariant tr signature /\
+    verify_with_label vk lab content signature /\
+    has_mls_signwithlabel_pred (lab, spred)
+  )
+  (ensures
+    (
+      get_signkey_usage vk == SigKey "MLS.LeafSignKey" empty ==>
+      spred.pred tr vk content
+    ) \/ (
+      (get_signkey_label vk) `can_flow tr` public 
+    )
+  )
+let bytes_invariant_verify_with_label #ci spred tr vk lab content signature =
+  let sign_content: sign_content_nt bytes = {
+    label = get_mls_label lab;
+    content = content;
+  } in
+  serialize_wf_lemma (sign_content_nt bytes) (bytes_invariant tr) sign_content
